finite map length

src/cbor/CBOR.Spec.FiniteMap.fst
@@ -140,3 +140,187 @@ let union (#t #u: Type) (s1 s2: fmap t u) : Pure (fmap t u)
   | _ -> s' x'
   ))
   (l1 `List.Tot.append` l2)
+
+let rec list_memP_extract
+  (#t: Type)
+  (x: t)
+  (l: list t)
+: Ghost (list t & list t)
+  (requires FStar.List.Tot.memP x l)
+  (ensures fun (ll, lr) ->
+    l == ll `List.Tot.append` (x :: lr)
+  )
+= let a :: q = l in
+  if FStar.StrongExcludedMiddle.strong_excluded_middle (a == x)
+  then ([], q)
+  else
+    let (ll, lr) = list_memP_extract x q in
+    (a :: ll, lr)
+
+let ghost_neq (#t: Type) (l2: t) : Tot (Ghost.erased (t -> bool)) =
+  FStar.Ghost.Pull.pull (fun l1 -> FStar.StrongExcludedMiddle.strong_excluded_middle (~ (l1 == l2)))
+
+let ghost_neq_equiv (#t: Type) (l2: t) (l1: t) : Lemma
+  (Ghost.reveal (ghost_neq l2) l1 <==> (~ (l1 == l2)))
+//  [SMTPat (Ghost.reveal (ghost_neq l2) l1)]
+= ()
+
+let rec list_length_filter
+  (#t: Type)
+  (f: t -> bool)
+  (l: list t)
+: Lemma
+  (List.Tot.length (List.Tot.filter f l) <= List.Tot.length l)
+  [SMTPat (List.Tot.length (List.Tot.filter f l))]
+= match l with
+  | [] -> ()
+  | _ :: q -> list_length_filter f q
+
+let rec list_memP_filter (#t: Type) (f: t -> bool) (l: list t) (x: t) : Lemma
+  (ensures List.Tot.memP x (List.Tot.filter f l) <==> List.Tot.memP x l /\ f x)
+  (decreases l)
+  [SMTPat (List.Tot.memP x (List.Tot.filter f l))]
+= match l with
+  | [] -> ()
+  | _ :: q -> list_memP_filter f q x
+
+let rec list_filter_eq_length
+  (#t: Type)
+  (f: t -> bool)
+  (l: list t)
+: Lemma
+  (requires (List.Tot.length (List.Tot.filter f l) == List.Tot.length l))
+  (ensures (List.Tot.filter f l == l))
+= match l with
+  | [] -> ()
+  | a :: q -> list_length_filter f q; list_filter_eq_length f q
+
+let rec list_memP_equiv_no_repeats // this is actually some form of the pigeon-hole principle
+  (#t: Type)
+  (l1 l2: list t)
+: Lemma
+  (requires (
+    List.Tot.no_repeats_p l1 /\
+    (forall x . List.Tot.memP x l1 <==> List.Tot.memP x l2) /\
+    List.Tot.length l1 >= List.Tot.length l2
+  ))
+  (ensures (
+    List.Tot.length l1 == List.Tot.length l2 /\
+    List.Tot.no_repeats_p l2
+  ))
+  (decreases l1)
+= match l1 with
+  | [] -> ()
+  | a :: q ->
+    let (ll, lr) = list_memP_extract a l2 in
+    List.Tot.append_length ll (a :: lr);
+    List.Tot.append_length ll lr;
+    let q2 = List.Tot.filter (ghost_neq a) (ll `List.Tot.append` lr) in
+    list_length_filter (ghost_neq a) (ll `List.Tot.append` lr);
+    let prf
+      (x: t)
+    : Lemma
+      (List.Tot.memP x q <==> List.Tot.memP x q2)
+    = list_memP_filter (ghost_neq a) (ll `List.Tot.append` lr) x;
+      List.Tot.append_memP ll lr x;
+      List.Tot.append_memP ll (a :: lr) x;
+      ghost_neq_equiv a x;
+      assert (Ghost.reveal (ghost_neq a) x <==> ~ (x == a));
+      assert (List.Tot.memP x q2 <==> (List.Tot.memP x ll \/ List.Tot.memP x lr) /\ Ghost.reveal (ghost_neq a) x);
+      assert (List.Tot.memP x q2 <==> (List.Tot.memP x ll \/ List.Tot.memP x lr) /\ ~ (x == a))
+    in
+    Classical.forall_intro prf;
+    list_memP_equiv_no_repeats q q2;
+    list_filter_eq_length (ghost_neq a) (ll `List.Tot.append` lr);
+    assert (q2 == ll `List.Tot.append` lr);
+    assert (List.Tot.no_repeats_p (a :: q2));
+    List.Tot.no_repeats_p_append_permut [] [] ll [a] lr
+
+#restart-solver
+let rec list_no_repeats_filter
+  (#key: Type)
+  (f: key -> bool)
+  (l: list key)
+: Lemma
+  (requires
+    List.Tot.no_repeats_p l
+  )
+  (ensures
+    List.Tot.no_repeats_p (List.Tot.filter f l)
+  )
+  [SMTPat (List.Tot.no_repeats_p (List.Tot.filter f l))]
+= match l with
+  | [] -> ()
+  | k :: q ->
+    list_no_repeats_filter f q
+
+let rec prune_list
+  (#key: Type)
+  (l: list key)
+: Ghost (list key)
+    (requires True)
+    (ensures (fun l' ->
+      List.Tot.length l >= List.Tot.length l' /\
+      List.Tot.no_repeats_p l' /\
+      (forall k . List.Tot.memP k l' <==> List.Tot.memP k l)     ))
+= match l with
+  | [] -> []
+  | k :: l' ->
+    let res =
+      k :: List.Tot.filter (ghost_neq k) (prune_list l')
+    in
+    list_no_repeats_filter (ghost_neq k) (prune_list l');
+    Classical.forall_intro (ghost_neq_equiv #key k);
+    res
+
+let length
+  (#t #u: Type)
+  (s: fmap t u)
+: GTot nat
+= let l = fmap_elim s in
+  List.Tot.length (prune_list l)
+
+let length_intro
+  (#t #u: Type)
+  (s: fmap t u)
+  (l: list t)
+: Lemma
+  (requires (
+    List.Tot.no_repeats_p l /\
+    (forall k . List.Tot.memP k l <==> Some? (get k s))
+  ))
+  (ensures (
+    length s == List.Tot.length l
+  ))
+= let l0 = prune_list (fmap_elim s) in
+  if List.Tot.length l0 >= List.Tot.length l
+  then list_memP_equiv_no_repeats l0 l
+  else list_memP_equiv_no_repeats l l0
+
+let length_empty
+  (t u: Type)
+: Lemma
+  (length (empty t u) == 0)
+  [SMTPat (length (empty t u))]
+= length_intro (empty t u) []
+
+let length_singleton
+  (#t #u: Type) (x: t) (elt: u) (eq: eq_elem_test x) (equ: eq_elem_test elt)
+: Lemma
+  (length (singleton x elt eq equ) == 1)
+  [SMTPat (length (singleton x elt eq equ))]
+= length_intro (singleton x elt eq equ) [x]
+
+let length_disjoint_union
+  (#t #u: Type) (s1 s2: fmap t u)
+: Lemma
+  (requires (disjoint s1 s2))
+  (ensures (
+    length (union s1 s2) == length s1 + length s2
+  ))
+= let l1 = prune_list (fmap_elim s1) in
+  let l2 = prune_list (fmap_elim s2) in
+  Classical.forall_intro (FStar.List.Tot.append_memP l1 l2);
+  List.Tot.no_repeats_p_append l1 l2;
+  List.Tot.append_length l1 l2;
+  length_intro (union s1 s2) (l1 `List.Tot.append` l2)
